perm_unsafe_lift/AnnExp.thy
@@ -1,0 +1,17 @@
+theory AnnExp
+  imports WTLemma
+begin
+  
+datatype ann_exp =
+  ConstAExp p_const
+  | OpAExp p_op
+  | VarAExp string var_val_ref
+  | PairAExp ann_exp ann_exp
+  | IfAExp ann_exp ann_exp ann_exp
+  | LamAExp string p_type ann_exp
+  | AppAExp ann_exp ann_exp    
+  
+    
+    
+end
+  
