perm_unsafe_lift/WellTypedAlt.thy
@@ -1,0 +1,236 @@
+theory WellTypedAlt
+  imports WTLemma
+begin
+  
+datatype wta_tag =
+  ConstRule
+  | OpRule
+  | VarRule
+  | PairRule
+  | IfRule
+  | LamRule
+  | AppRule
+  | WeakPostRule wta_tag
+  | StrReqRule wta_tag
+  | WeakReqRule wta_tag
+    
+fun well_typed_alt :: "wta_tag \<Rightarrow> pt_env \<Rightarrow> perm_use_env \<Rightarrow> p_exp \<Rightarrow> p_type \<Rightarrow> perm_use_env \<Rightarrow> perm_use_env \<Rightarrow> bool" where
+  "well_typed_alt ConstRule env r_s1 e tau r_s2 rx = (\<exists> c. e = ConstExp c \<and> tau \<in> const_type c \<and> r_s2 = r_s1 \<and> rx = empty_use_env)"
+| "well_typed_alt OpRule env r_s1 e tau r_s2 rx = (\<exists> xop. e = OpExp xop \<and> tau = op_type xop \<and> r_s2 = r_s1 \<and> rx = empty_use_env)"
+| "well_typed_alt VarRule env r_s1 e tau r_s2 rx = (\<exists> x v tau_x. e = VarExp x v \<and> env (deref_name x v) = Some tau \<and>
+    env x = Some tau_x \<and> var_val_type v tau tau_x \<and> leq_use_env (ereq_use_env x tau_x) r_s1 \<and> r_s2 = diff_use_env r_s1 (ereq_use_env x tau_x) \<and>
+    rx = diff_use_env (ereq_use_env x tau_x) (ereq_use_env x tau_x))"
+| "well_typed_alt PairRule env r_s1 e tau r_s3 rf = (\<exists> e1 e2 t1 t2 r r_s2 rx1 rx2. e = PairExp e1 e2 \<and>
+    tau = PairTy t1 t2 r \<and> well_typed env r_s1 e1 t1 r_s2 rx1 \<and> well_typed env r_s2 e2 t2 r_s3 rx2 \<and>
+    leq_use_env (lift_use_env rx1 r) r_s3 \<and> leq_use_env (lift_use_env rx2 r) r_s3 \<and> aff_leq (max_aff (req_type t1) (req_type t2)) r \<and>
+    disj_use_env (lift_use_env rx1 r) (lift_use_env rx2 r) \<and>
+    rf = pair_req (comp_use_env (lift_use_env rx1 r) (lift_use_env rx2 r)) empty_use_env tau
+  )"  
+| "well_typed_alt IfRule env r_s1 e tau r_s3 rx = (\<exists> e1 e2 e3 rx' r_s2 rx1 rx2. e = IfExp e1 e2 e3 \<and>
+    well_typed env r_s1 e1 BoolTy r_s2 rx' \<and> well_typed env r_s2 e2 tau r_s3 rx1 \<and> well_typed env r_s2 e3 tau r_s3 rx2 \<and>
+    rx = comp_use_env rx1 rx2)"
+| "well_typed_alt LamRule env r_s1 ex tau r_s2 rx = (\<exists> x e t1 t2 r a r_end r_s'. ex = LamExp x e \<and>
+    tau = FunTy t1 t2 r a \<and> x \<notin> ref_vars e \<and>
+    well_typed (add_env env x t1) (add_use_env rx x r) e t2 r_s' r_end \<and> aff_use_env rx a \<and>
+    leq_use_env rx r_s1 \<and> r_s2 = r_s1)"
+| "well_typed_alt AppRule env r_s1 e tau r_sf rx = (\<exists> e1 e2 t1 r a r_s2 rx1 rx2 r_s3. e = AppExp e1 e2 \<and>
+    well_typed env r_s1 e1 (FunTy t1 tau r a) r_s2 rx1 \<and> well_typed env r_s2 e2 t1 r_s3 rx2 \<and>
+    r_sf = diff_use_env r_s3 (comp_use_env rx1 (lift_use_env rx2 r)) \<and> (*r \<noteq> NoPerm \<and>*) (*safe_use_lift rx2 r \<and>
+    safe_type t1 r \<and>*) leq_use_env (comp_use_env rx1 (lift_use_env rx2 r)) r_s3 \<and>
+    disj_use_env rx1 (lift_use_env rx2 r) \<and> leq_use_env rx r_sf \<and> 
+    rx = app_req rx1 rx2 r tau empty_use_env
+  )"
+| "well_typed_alt (WeakPostRule tag) env r_s1 e tau r_s2 rx = (\<exists> r_c. well_typed_alt tag env r_s1 e tau r_c rx \<and>
+    leq_use_env rx r_s2 \<and> leq_use_env r_s2 r_c)"
+| "well_typed_alt (StrReqRule tag) env r_s1 e tau r_s2 rx = (\<exists> rx'. well_typed_alt tag env r_s1 e tau r_s2 rx' \<and>
+    leq_use_env rx' rx \<and> leq_use_env rx r_s2)"
+| "well_typed_alt (WeakReqRule tag) env r_s1 e tau r_s2 rx = (\<exists> r_se r_xe r_ex. well_typed_alt tag env r_s1 e tau r_se r_xe \<and>
+    r_s2 = diff_use_env r_se r_ex \<and> rx = diff_use_env r_xe r_ex \<and> leq_use_env r_ex r_s1)"
+  
+  
+lemma well_typed_equiv1: "\<lbrakk> well_typed env r_s1 e tau r_s2 rx \<rbrakk> \<Longrightarrow> (\<exists> tag. well_typed_alt tag env r_s1 e tau r_s2 rx)"  
+  apply (induct e arbitrary: env r_s1 r_s2 tau rx)
+        apply (auto)
+    (* const case *)
+        apply (rule_tac x="StrReqRule (WeakPostRule ConstRule)" in exI)
+        apply (auto)
+         apply (rule_tac leq_empty_use_env)
+        apply (rule_tac leq_empty_use_env)
+    (* op case *)
+       apply (rule_tac x="StrReqRule (WeakPostRule OpRule)" in exI)
+       apply (auto)
+        apply (rule_tac leq_empty_use_env)
+       apply (rule_tac leq_empty_use_env)
+    (* var case *)
+      apply (rule_tac x="WeakPostRule (StrReqRule (WeakReqRule VarRule))" in exI)
+      apply (auto)
+      apply (rule_tac x="diff_use_env (diff_use_env r_s1 (ereq_use_env x1a tau_x)) r_ex" in exI)
+      apply (auto)
+       apply (rule_tac x="diff_use_env (diff_use_env (ereq_use_env x1a tau_x) (ereq_use_env x1a tau_x)) r_ex" in exI)
+       apply (auto)
+        apply (rule_tac lhs_fold_dcl_use_env)
+        apply (simp)
+       apply (rule_tac r_sb="r_s2" in trans_leq_use_env)
+        apply (rule_tac rhs_fold_dcl_use_env)
+        apply (simp_all)
+      apply (rule_tac rhs_fold_dcl_use_env)
+      apply (simp)
+    (* pair case *)
+     apply (rule_tac x="WeakPostRule (StrReqRule (WeakReqRule PairRule))" in exI)
+     apply (auto)
+     apply (rule_tac x="diff_use_env r_s3 r_ex" in exI)
+     apply (auto)
+     apply (rule_tac x="pair_req (comp_use_env (lift_use_env rx1 r) (lift_use_env rx2 r)) r_ex (PairTy t1 t2 r)" in exI)
+     apply (auto)
+      apply (rule_tac x="r_s3" in exI)
+      apply (rule_tac x="pair_req (comp_use_env (lift_use_env rx1 r) (lift_use_env rx2 r)) empty_use_env (PairTy t1 t2 r)" in exI)
+      apply (auto)
+      apply (rule_tac x="r_ex" in exI)
+      apply (auto)
+      apply (simp add: pair_req_def)
+      apply (auto)
+       apply (simp add: diff_empty_use_env1)
+      apply (simp add: diff_empty_use_env2)
+     apply (rule_tac r_sb="r_s2" in trans_leq_use_env)
+      apply (auto)
+    (* if case *)
+    apply (rule_tac x="IfRule" in exI)
+    apply (auto)
+    (* lam case *)
+   apply (rule_tac x="WeakPostRule (StrReqRule (WeakReqRule LamRule))" in exI)
+   apply (auto)
+   apply (rule_tac x="diff_use_env r_s1 r_ex" in exI)
+   apply (auto)
+   apply (rule_tac x="diff_use_env rxa r_ex" in exI)
+   apply (auto)
+   apply (rule_tac r_sb="r_s2" in trans_leq_use_env)
+    apply (auto)
+    (* app case *)
+  apply (rule_tac x="WeakPostRule (StrReqRule (WeakReqRule AppRule))" in exI)
+  apply (auto)
+  apply (rule_tac x="diff_use_env (diff_use_env r_s3 (comp_use_env rx1 (lift_use_env rx2 r))) r_ex" in exI)
+  apply (auto)
+   apply (rule_tac x="app_req rx1 rx2 r tau r_ex" in exI)
+   apply (auto)
+    apply (rule_tac x="diff_use_env r_s3 (comp_use_env rx1 (lift_use_env rx2 r))" in exI)
+    apply (rule_tac x="app_req rx1 rx2 r tau empty_use_env" in exI)
+    apply (auto)
+     apply (rule_tac x="t1" in exI)
+     apply (rule_tac x="r" in exI)
+     apply (rule_tac x="a" in exI)
+     apply (rule_tac x="r_s2a" in exI)
+     apply (rule_tac x="rx1" in exI)
+     apply (auto)
+     apply (rule_tac x="rx2" in exI)
+     apply (rule_tac x="r_s3" in exI)
+     apply (auto)
+     apply (simp add: app_req_def)
+     apply (auto)
+      apply (rule_tac leq_empty_use_env)
+     apply (rule_tac dist_diff_leq_use_env_gen)
+      apply (rule_tac r_sb="comp_use_env rx1 (lift_use_env rx2 r)" in trans_leq_use_env)
+       apply (simp)
+      apply (rule_tac dist_comp_leq_use_env)
+       apply (rule_tac self_comp_leq_use_env1)
+      apply (rule_tac comp_leq_use_env2)
+      apply (rule_tac self_lift_leq_use_env)
+     apply (rule_tac self_comp_leq_use_env1)
+    apply (rule_tac x="r_ex" in exI)
+    apply (auto)
+    apply (simp add: app_req_def)
+    apply (auto)
+     apply (simp add: diff_empty_use_env1)
+    apply (simp add: comp_empty_use_env2)
+    apply (simp add: diff_comp_use_env)
+   apply (rule_tac r_sb="r_s2" in trans_leq_use_env)
+    apply (rule_tac rhs_fold_dcl_use_env)
+    apply (simp_all)
+  apply (rule_tac rhs_fold_dcl_use_env)
+  apply (simp)
+  done
+   
+lemma well_typed_equiv2: "\<lbrakk> well_typed_alt tag env r_s1 e tau r_s2 rx \<rbrakk> \<Longrightarrow> well_typed env r_s1 e tau r_s2 rx"      
+  apply (induct tag arbitrary: env r_s1 e tau r_s2 rx)  
+           apply (auto)
+    (* const + op case *)
+             apply (rule_tac id_leq_use_env)
+            apply (rule_tac leq_empty_use_env)
+           apply (rule_tac id_leq_use_env)
+          apply (rule_tac leq_empty_use_env)
+    (* var case *)
+         apply (rule_tac x="empty_use_env" in exI)
+         apply (auto)
+           apply (rule_tac dist_diff_leq_use_env_gen)
+            apply (rule_tac id_leq_use_env)
+           apply (rule_tac dist_comp_leq_use_env)
+            apply (rule_tac id_leq_use_env)
+           apply (rule_tac leq_empty_use_env)
+          apply (rule_tac dist_diff_leq_use_env_gen)
+           apply (simp)
+          apply (rule_tac id_leq_use_env)
+         apply (rule_tac leq_empty_use_env)
+        apply (rule_tac dist_diff_leq_use_env_gen)
+         apply (rule_tac id_leq_use_env)
+        apply (rule_tac self_comp_leq_use_env1)
+    (* pair case *)
+       apply (rule_tac x="r_s2a" in exI)
+       apply (rule_tac x="r_s2" in exI)
+       apply (rule_tac x="rx1" in exI)
+       apply (auto)
+       apply (rule_tac x="rx2" in exI)
+       apply (auto)
+       apply (rule_tac x="empty_use_env" in exI)
+       apply (auto)
+          apply (simp add: diff_empty_use_env2)
+          apply (rule_tac id_leq_use_env)
+         apply (simp add: pair_req_def)
+         apply (auto)
+          apply (rule_tac leq_empty_use_env)
+         apply (rule_tac diff_leq_use_env)
+         apply (rule_tac dist_comp_leq_use_env)
+          apply (simp_all)
+        apply (rule_tac leq_empty_use_env)
+       apply (simp add: pair_req_def)
+       apply (auto)
+        apply (rule_tac leq_empty_use_env)
+       apply (rule_tac id_leq_use_env)
+    (* lam case *)
+      apply (rule_tac x="rx" in exI)
+      apply (auto)
+      apply (rule_tac x="empty_use_env" in exI)
+      apply (auto)
+         apply (simp add: diff_empty_use_env2)
+         apply (rule_tac id_leq_use_env)
+       apply (rule_tac leq_empty_use_env)
+      apply (rule_tac self_diff_leq_use_env)
+    (* app case *)
+     apply (rule_tac x="t1" in exI)
+     apply (rule_tac x="r" in exI)
+     apply (rule_tac x="a" in exI)
+     apply (rule_tac x="r_s2a" in exI)
+     apply (rule_tac x="rx1" in exI)
+     apply (auto)
+     apply (rule_tac x="rx2" in exI)
+     apply (rule_tac x="r_s3" in exI)
+     apply (auto)
+     apply (rule_tac x="empty_use_env" in exI)
+     apply (auto)
+       apply (rule_tac dist_diff_leq_use_env_gen)
+        apply (rule_tac id_leq_use_env)
+       apply (rule_tac dist_comp_leq_use_env)
+        apply (rule_tac id_leq_use_env)
+       apply (rule_tac leq_empty_use_env)
+      apply (rule_tac leq_empty_use_env)
+     apply (rule_tac id_leq_use_env)
+    (* post weakening case *)
+    apply (rule_tac r_c="r_c" in well_typed_decr_end_perm)
+      apply (auto)
+    (* req strengthening case *)
+   apply (rule_tac rx="rx'" in well_typed_incr_req)
+     apply (auto)
+    (* req weakening case *)
+  apply (rule_tac well_typed_diff_end_perm)
+   apply (auto)
+  done
+    
+end
